state main theorems for spinlock correctness
with cheats and yet without exclusive banks

examples/spinlock/spinlockScript.sml
@@ -12,7 +12,11 @@ val _ = lift_da_and_store_mc_riscv
           "spinlock.da"
           ((Arbnum.fromInt 0), (Arbnum.fromInt 0x1000000));
 
-open bir_promisingTheory;
+open bir_promisingTheory rich_listTheory listTheory arithmeticTheory;
+
+(*
+ * characterisation of fulfil and promise rules
+ *)
 
 Definition is_fulfil_def:
   is_fulfil cid t system1 system2 =
@@ -22,6 +26,13 @@ Definition is_fulfil_def:
     /\ FILTER (λt'. t' <> t) st.bst_prom = st'.bst_prom
     /\ MEM t st.bst_prom
 End
+
+Theorem is_fulfil_MEM_bst_prom:
+  is_fulfil cid t system1 system2
+  ==> ?p st. Core cid p st IN system1  /\ MEM t st.bst_prom
+Proof
+  fs[is_fulfil_def] >> metis_tac[]
+QED
 
 Definition is_promise_def:
   is_promise cid t M M' system1 system2 =
@@ -33,8 +44,12 @@ Definition is_promise_def:
     /\ st'.bst_prom = st.bst_prom ++ [t]
 End
 
+(*
+ * Defintion of traces
+ *)
+
 Definition parstep_nice_def:
-  parstep_nice (sys1, M1) (sys2, M2) = parstep sys1 M1 sys2 M2
+  parstep_nice s1 s2 = parstep (FST s1) (SND s1) (FST s2) (SND s2)
 End
 
 (* set of all traces using bir_multicore$gen_traces *)
@@ -42,10 +57,372 @@ Definition par_traces_def:
   par_traces = gen_traces parstep_nice
 End
 
-Theorem par_trace_promise_preceeds_fulfil:
-  !i tr cid t.
-  tr IN par_traces
+Theorem par_traces_ind:
+  !P. (!s. P [s])
+  /\ (!s2 s1 t. P (t ++ [s1]) /\ parstep_nice s1 s2 ==> P (t ++ [s1; s2]))
+  ==> !tr. tr IN par_traces ==> P tr
+Proof
+  fs[par_traces_def,bir_multicoreTheory.gen_traces_def]
+  >> ntac 2 strip_tac
+  >> `!ps tr. is_gen_trace ps tr ==> ps = parstep_nice ==> P tr` by (
+    ho_match_mp_tac bir_multicoreTheory.is_gen_trace_ind
+    >> fs[]
+  )
+  >> fs[]
+QED
+
+Theorem is_gen_trace_NOT_NULL:
+  !R s. is_gen_trace R s ==> ~NULL s
+Proof
+  ho_match_mp_tac bir_multicoreTheory.is_gen_trace_ind
+  >> fs[NULL_EQ]
+QED
+
+Theorem is_gen_trace_EL:
+  !R s. is_gen_trace R s ==> !i. SUC i < LENGTH s ==> R (EL i s) (EL (SUC i) s)
+Proof
+  ho_match_mp_tac bir_multicoreTheory.is_gen_trace_ind
+  >> rw[]
+  >> qmatch_assum_rename_tac `SUC i < LENGTH t + 2`
+  >> Cases_on `SUC i < LENGTH t`
+  >- (
+    first_x_assum $ qspec_then `i` mp_tac
+    >> fs[EL_APPEND1]
+  )
+  >> fs[NOT_LESS,LESS_OR_EQ]
+  >- (
+    `i = LENGTH t` by fs[]
+    >> pop_assum $ fs o single
+    >> fs[EL_APPEND1,EL_APPEND2]
+  )
+  >> first_x_assum $ qspec_then `i` mp_tac
+  >> fs[EL_APPEND1,EL_APPEND2]
+QED
+
+(*
+ * well-formed traces and implications of well-formedness
+ *)
+
+(* well-formedness of Cores: the cid is unique *)
+Definition wf_sys_def:
+  wf_sys (sys : core_t -> bool) =
+    !cid p st p' st'.
+    Core cid p st IN sys /\ Core cid p' st' IN sys
+    ==> p = p' /\ st = st'
+End
+
+Theorem parstep_nice_wf_sys:
+  !s1 s2. wf_sys $ FST s1
+  /\ parstep_nice s1 s2
+  ==> wf_sys $ FST s2
+Proof
+  `!s1 m1 s2 m2. parstep s1 m1 s2 m2 ==> wf_sys s1 ==> wf_sys s2` by (
+    ho_match_mp_tac bir_promisingTheory.parstep_ind
+    >> rpt strip_tac
+    >> fs[wf_sys_def,AND_IMP_INTRO]
+    >> rw[]
+    >> first_x_assum dxrule_all >> rw[]
+  )
+  >> ntac 2 Cases >> fs[parstep_nice_def]
+  >> metis_tac[]
+QED
+
+Definition empty_prom_def:
+  empty_prom s = !cid p st. Core cid p st IN s ==> NULL st.bst_prom
+End
+
+(* well-formed traces are certified and thread id's are unique identifiers *)
+Definition wf_trace_def:
+  wf_trace tr <=> tr IN par_traces /\ wf_sys $ FST $ HD tr
+    /\ NULL $ SND $ HD tr /\ empty_prom $ FST $ HD tr
+End
+
+Theorem wf_trace_NOT_NULL:
+  !tr. wf_trace tr ==> ~NULL tr
+Proof
+  rw[wf_trace_def,par_traces_def,bir_multicoreTheory.gen_traces_def]
+  >> imp_res_tac is_gen_trace_NOT_NULL
+QED
+
+Theorem wf_trace_parstep_EL:
+  !tr i. wf_trace tr /\ SUC i < LENGTH tr ==> parstep_nice (EL i tr) (EL (SUC i) tr)
+Proof
+ fs[is_gen_trace_EL,wf_trace_def,par_traces_def,bir_multicoreTheory.gen_traces_def]
+QED
+
+Theorem par_traces_wf_sys_monotone:
+  !tr i.
+    tr IN par_traces /\ wf_sys $ FST $ HD tr
+    /\ i < LENGTH tr ==> wf_sys $ FST $ EL i tr
+Proof
+  `!ps tr. is_gen_trace ps tr ==>
+    ps = parstep_nice /\ wf_sys (FST (HD tr)) ==>
+     !i. i < LENGTH tr ==> wf_sys (FST (EL i tr))` by (
+    ho_match_mp_tac bir_multicoreTheory.is_gen_trace_ind
+    >> rw[]
+    >- (qmatch_assum_rename_tac `i < 1` >> Cases_on `i` >> fs[])
+    >> qmatch_assum_rename_tac `i < LENGTH t + 2`
+    >> Cases_on `NULL t`
+    >- (
+      fs[NULL_EQ,EL_APPEND1,EL_APPEND2]
+      >> fs o single $
+        (REWRITE_CONV [GSYM COUNT_LIST_COUNT,
+        GSYM pred_setTheory.IN_COUNT]
+        THENC EVAL) ``n < (2 : num)``
+      >> drule_all parstep_nice_wf_sys
+      >> fs[]
+    )
+    >> gs[Excl"EL",Excl"EL_restricted",GSYM EL,EL_APPEND1,GSYM LENGTH_NOT_NULL]
+    >> Cases_on `i < LENGTH t`
+    >- (
+      `i < LENGTH t + 1` by fs[]
+      >> first_x_assum drule
+      >> fs[EL_APPEND1]
+    )
+    >> gvs[EL_APPEND2,NOT_LESS,LESS_OR_EQ,EL_APPEND1]
+    >> first_x_assum $ qspec_then `LENGTH t` mp_tac
+    >> fs[EL_APPEND2]
+    >> `i = SUC $ LENGTH t` by fs[NOT_LESS,LESS_OR_EQ]
+    >> rw[EL_APPEND1]
+    >> dxrule_all parstep_nice_wf_sys
+    >> fs[]
+  )
+  >> fs[par_traces_def,bir_multicoreTheory.gen_traces_def]
+QED
+
+Theorem wf_trace_wf_sys:
+  !tr cid p st p' st' i. wf_trace tr
+  /\ Core cid p st IN FST (EL i tr)
+  /\ Core cid p' st' IN FST (EL i tr)
+  /\ i < LENGTH tr
+  ==> p = p' /\ st = st'
+Proof
+  rpt gen_tac >> strip_tac
+  >> fs[wf_trace_def]
+  >> drule_all par_traces_wf_sys_monotone
+  >> simp[wf_sys_def]
+  >> disch_then $ dxrule_all
+  >> fs[]
+QED
+
+Theorem wf_trace_is_promise_MEM_trace:
+  !tr cid t i M s. wf_trace tr
+  /\ is_promise cid t (SND $ EL i tr) M (FST $ EL i tr) s
+  /\ i < LENGTH tr
+  ==>  SUC i < LENGTH tr /\ M = SND $ EL (SUC i) tr /\ s = FST $ EL (SUC i) tr
+Proof
+  cheat
+QED
+
+Theorem wf_trace_is_fulfil_MEM_trace:
+  !tr cid t i s. wf_trace tr
+  /\ is_fulfil cid t (FST $ EL i tr) s
+  /\ i < LENGTH tr
+  ==>  SUC i < LENGTH tr /\ s = FST $ EL (SUC i) tr
+Proof
+  cheat
+QED
+
+(* only one fulfil happens at a time *)
+Theorem is_fulfil_same:
+  !tr cid cid' t t' i. wf_trace tr
+  /\ is_fulfil cid t (FST $ EL i tr) (FST $ EL (SUC i) tr)
+  /\ is_fulfil cid' t' (FST $ EL i tr) (FST $ EL (SUC i) tr)
   /\ SUC i < LENGTH tr
+  ==> cid = cid' /\ t = t'
+Proof
+  cheat
+QED
+
+(* only one promise happens at a time *)
+Theorem is_promise_same:
+  !tr cid cid' t t' i. wf_trace tr
+  /\ is_promise cid t (SND $ EL i tr) (SND $ EL (SUC i) tr)
+    (FST $ EL i tr) (FST $ EL (SUC i) tr)
+  /\ is_promise cid' t' (SND $ EL i tr) (SND $ EL (SUC i) tr)
+    (FST $ EL i tr) (FST $ EL (SUC i) tr)
+  /\ SUC i < LENGTH tr
+  ==> cid = cid' /\ t = t'
+Proof
+  cheat
+QED
+
+(* same core id occurs in next step in the trace *)
+Theorem wf_trace_cid_forward1:
+  !tr i cid p st. wf_trace tr /\ Core cid p st IN FST (EL i tr)
+  /\ SUC i < LENGTH tr
+  ==> ?p st. Core cid p st IN FST (EL (SUC i) tr)
+Proof
+  cheat
+QED
+
+(* same core id occurs later in the trace *)
+Theorem wf_trace_cid_forward:
+  !j tr i cid p st. wf_trace tr /\ Core cid p st IN FST (EL i tr)
+  /\ i <= j /\ j < LENGTH tr
+  ==> ?p st. Core cid p st IN FST (EL j tr)
+Proof
+  Induct >> rw[] >> fs[] >- goal_assum drule
+  >> dxrule_then strip_assume_tac $ iffLR LESS_OR_EQ
+  >- (
+    first_x_assum $ drule_then dxrule
+    >> rw[]
+    >> drule_then irule wf_trace_cid_forward1
+    >> rpt $ goal_assum $ drule_at Any
+  )
+  >> gvs[] >> goal_assum drule
+QED
+
+Theorem wf_trace_cid_backward1:
+  !i tr cid p st. wf_trace tr /\ Core cid p st IN FST (EL (SUC i) tr)
+  /\ SUC i < LENGTH tr
+  ==> ?p st. Core cid p st IN FST (EL i tr)
+Proof
+  cheat
+QED
+
+Theorem wf_trace_cid_backward:
+  !i j tr cid p st. wf_trace tr /\ Core cid p st IN FST (EL j tr)
+  /\ i <= j /\ j < LENGTH tr
+  ==> ?p st. Core cid p st IN FST (EL i tr)
+Proof
+  ntac 2 gen_tac >> Induct_on `j - i`
+  >> rw[] >> fs[PULL_FORALL,AND_IMP_INTRO]
+  >- (gvs[LESS_OR_EQ] >- goal_assum drule)
+  >> drule_then irule wf_trace_cid_backward1
+  >> qpat_x_assum `_ = _ - _:num` $ assume_tac o REWRITE_RULE[SUB_LEFT_EQ]
+  >> gvs[]
+  >> first_x_assum $ rev_drule_at_then Any irule
+  >> goal_assum $ rev_drule_at Any
+  >> fs[]
+QED
+
+(* a thread id occurs in all states *)
+Theorem wf_trace_cid:
+  !tr cid p st i j. wf_trace tr /\ Core cid p st IN FST (EL i tr)
+  /\ i < LENGTH tr /\ j < LENGTH tr
+  ==> ?p st. Core cid p st IN FST (EL j tr)
+Proof
+  rw[]
+  >> Cases_on `i <= j`
+  >- (
+    drule_then irule wf_trace_cid_forward
+    >> rpt $ goal_assum $ drule_at Any
+  )
+  >> drule_then irule wf_trace_cid_backward
+  >> goal_assum $ rev_drule_at Any
+  >> fs[]
+QED
+
+(* memory is monotonic only ever increases, at most by one *)
+
+Theorem parstep_nice_memory_imp:
+  !s1 s2. parstep_nice s1 s2
+  ==> SND s1 = SND s2 \/ ?m. SND s2 = SND s1 ++ [m]
+Proof
+  fs[par_traces_def,bir_multicoreTheory.gen_traces_def,parstep_nice_def,pairTheory.FORALL_PROD]
+  >> rw[bir_promisingTheory.cstep_cases,bir_promisingTheory.parstep_cases]
+  >> disj2_tac
+  >> irule_at Any EQ_REFL
+QED
+
+(* certified traces have empty promises in the last state *)
+
+Theorem wf_trace_LAST_NULL_bst_prom:
+  !tr cid p st. wf_trace tr
+  /\ Core cid p st IN FST $ LAST tr
+  ==> NULL st.bst_prom
+Proof
+  cheat
+QED
+
+(* a promise entails lower bound of future memory length *)
+
+Theorem is_promise_LENGTH_SND_EL:
+  !i j tr cid t. wf_trace tr
+  /\ is_promise cid t (SND $ EL i tr) (SND $ EL (SUC i) tr)
+    (FST $ EL i tr) (FST $ EL (SUC i) tr)
+  /\ SUC i <= j /\ j < LENGTH tr
+  ==> t <= LENGTH (SND $ EL j tr)
+Proof
+  rpt gen_tac
+  >> Induct_on `j - SUC i`
+  >- (rw[is_promise_def] >> gs[LESS_OR_EQ])
+  >> rw[SUB_LEFT_EQ]
+  >> first_x_assum $ rev_drule_at Any
+  >> disch_then $ rev_drule_at Any
+  >> disch_then $ qspec_then `v + SUC i` assume_tac
+  >> `SUC $ v + SUC i < LENGTH tr` by fs[]
+  >> drule_all_then assume_tac wf_trace_parstep_EL
+  >> dxrule_then strip_assume_tac parstep_nice_memory_imp
+  >> gs[]
+  >> `SUC i + SUC v = SUC $ v + SUC i` by fs[]
+  >> pop_assum $ fs o single
+QED
+
+(* a promise is only promised once *)
+
+Theorem is_promise_once:
+  !i j tr cid cid' t. wf_trace tr
+  /\ is_promise cid t (SND $ EL i tr) (SND $ EL (SUC i) tr)
+    (FST $ EL i tr) (FST $ EL (SUC i) tr)
+  /\ i < j /\ SUC j < LENGTH tr
+  ==> ~is_promise cid' t (SND $ EL j tr) (SND $ EL (SUC j) tr)
+    (FST $ EL j tr) (FST $ EL (SUC j) tr)
+Proof
+  rpt strip_tac
+  >> rev_drule_at Any is_promise_LENGTH_SND_EL
+  >> disch_then $ rev_drule_at_then Any assume_tac
+  >> first_assum $ qspec_then `j` assume_tac
+  >> first_x_assum $ qspec_then `SUC j` assume_tac
+  >> dxrule_then strip_assume_tac $ iffLR is_promise_def
+  >> gvs[]
+QED
+
+Theorem clstep_bst_prom_EQ:
+  clstep p cid st M [] st' ==> st.bst_prom = st'.bst_prom
+Proof
+  rw[bir_promisingTheory.clstep_cases]
+  >> gvs[bir_programTheory.bir_state_t_accfupds,bir_programTheory.bir_exec_stmt_def,bir_programTheory.bir_exec_stmtE_def,bir_programTheory.bir_exec_stmt_cjmp_def,AllCaseEqs(),bir_programTheory.bir_state_set_typeerror_def,stmt_generic_step_def]
+  >> cheat
+QED
+
+(* a fulfil has an earlier promise *)
+
+Theorem NOT_is_promise_NOT_MEM_bst_prom:
+  !i tr cid p st p' st' t. wf_trace tr
+  /\ ~is_promise cid t (SND $ EL i tr) (SND $ EL (SUC i) tr)
+    (FST $ EL i tr) (FST $ EL (SUC i) tr)
+  /\ SUC i < LENGTH tr
+  /\ Core cid p st IN FST $ EL i tr
+  /\ ~MEM t st.bst_prom
+  /\ Core cid p' st' IN FST $ EL (SUC i) tr
+  ==> ~MEM t st'.bst_prom
+Proof
+  rw[]
+  >> drule_all_then strip_assume_tac wf_trace_parstep_EL
+  >> fs[parstep_nice_def,bir_promisingTheory.parstep_cases]
+  >> Cases_on `cid = cid'`
+  >- (
+    pop_assum $ fs o single
+    >> drule_then (dxrule_then drule) wf_trace_wf_sys
+    >> rw[]
+    >> fs[is_promise_def,DISJ_EQ_IMP]
+    >> first_x_assum drule
+    >> fs[AND_IMP_INTRO,AC CONJ_ASSOC CONJ_COMM,bir_promisingTheory.cstep_cases]
+    >- (dxrule_then assume_tac clstep_bst_prom_EQ >> fs[])
+    >> rpt strip_tac
+    >> Cases_on `msg`
+    >> gvs[AND_IMP_INTRO,mem_msg_t_val,mem_msg_t_loc,mem_msg_t_cid]
+    >> cheat
+  )
+  >> `Core cid p st IN FST $ EL (SUC i) tr` by fs[EQ_SYM_EQ]
+  >> dxrule wf_trace_wf_sys
+  >> ntac 2 $ disch_then dxrule >> strip_tac >> gs[]
+QED
+
+Theorem is_fulfil_is_promise:
+  !i tr cid t. wf_trace tr /\ SUC i < LENGTH tr
   /\ is_fulfil cid t (FST $ EL i tr) (FST $ EL (SUC i) tr)
   ==> ?j. j < i
     /\ is_promise cid t (SND $ EL j tr) (SND $ EL (SUC j) tr)
@@ -53,11 +430,320 @@ Theorem par_trace_promise_preceeds_fulfil:
 Proof
   rpt strip_tac
   >> CCONTR_TAC
-  >> `?p st. Core cid p st IN FST $ EL i tr  /\ MEM t st.bst_prom` by (
-    fs[is_fulfil_def] >> metis_tac[]
-  )
   >> fs[DISJ_EQ_IMP]
+  >> `!j p st. j <= i /\ Core cid p st IN FST $ EL j tr ==> ~MEM t st.bst_prom` by (
+    Induct
+    >- (
+      rw[] >> fs[wf_trace_def,empty_prom_def]
+      >> strip_tac
+      >> res_tac
+      >> gs[NULL_EQ]
+    )
+    >> rw[] >> gs[]
+    >> `j < i` by fs[]
+    >> first_x_assum $ dxrule_then assume_tac
+    >> drule_then drule wf_trace_cid_backward1
+    >> rw[]
+    >> first_x_assum $ drule_then assume_tac
+    >> drule_then drule NOT_is_promise_NOT_MEM_bst_prom
+    >> rpt $ disch_then $ drule_at Any
+    >> fs[]
+  )
+  >> fs[is_fulfil_def]
+  >> first_x_assum $ rev_drule_at Any
+  >> fs[]
+QED
+
+(* a promise has a succeeding fulfil *)
+
+Theorem NOT_is_fulfil_MEM_bst_prom:
+  !i tr cid p st p' st' t. wf_trace tr /\ SUC i < LENGTH tr
+  /\ ~is_fulfil cid t (FST $ EL i tr) (FST $ EL (SUC i) tr)
+  /\ Core cid p st IN FST $ EL i tr
+  /\ MEM t st.bst_prom
+  /\ Core cid p' st' IN FST $ EL (SUC i) tr
+  ==> MEM t st'.bst_prom
+Proof
+  rw[]
+  >> drule_all_then strip_assume_tac wf_trace_parstep_EL
+  >> fs[parstep_nice_def,bir_promisingTheory.parstep_cases,is_fulfil_def,DISJ_EQ_IMP]
+  >> Cases_on `cid = cid'`
+  >- (
+    pop_assum $ fs o single
+    >> drule_then (dxrule_then drule) wf_trace_wf_sys
+    >> rw[]
+    >> fs[bir_promisingTheory.cstep_cases]
+    >> drule_then assume_tac clstep_bst_prom_EQ
+    >> fs[]
+  )
+  >> first_x_assum $ rev_drule_then drule
+  >> `Core cid p st IN FST $ EL (SUC i) tr` by fs[EQ_SYM_EQ]
+  >> dxrule wf_trace_wf_sys
+  >> ntac 2 $ disch_then dxrule >> strip_tac >> gs[]
+QED
+
+Theorem is_promise_is_fulfil:
+  !i j tr cid t. wf_trace tr /\ SUC i < LENGTH tr
+  /\ is_promise cid t (SND $ EL i tr) (SND $ EL (SUC i) tr)
+    (FST $ EL i tr) (FST $ EL (SUC i) tr)
+  ==> ?j. i < j
+    /\ is_fulfil cid t (FST $ EL j tr) (FST $ EL (SUC j) tr)
+Proof
+  rpt strip_tac
+  >> CCONTR_TAC
+  >> fs[DISJ_EQ_IMP]
+  >> `!j p st. i < j /\ Core cid p st IN FST $ EL j tr ==> MEM t st.bst_prom` by (
+    (* TODO reverse induction analogue to is_fulfil_is_promise *)
+    cheat
+    (* NOT_is_fulfil_MEM_bst_prom *)
+  )
+  >> `?p st. Core cid p st IN FST $ LAST tr` by (
+    fs[is_promise_def,GSYM LENGTH_NOT_NULL,GSYM NULL_EQ,LAST_EL]
+    >> drule_then irule wf_trace_cid_forward
+    >> fs[]
+    >> goal_assum $ drule_at Any
+    >> fs[]
+  )
+  >> drule_all wf_trace_LAST_NULL_bst_prom
+  >> gs[GSYM LENGTH_NOT_NULL,GSYM NULL_EQ,LAST_EL]
+  >> first_x_assum $ drule_at Any
+  >> rw[LENGTH_NOT_NULL,MEM_SPLIT,NOT_NULL_MEM]
+  >> goal_assum drule
+QED
+
+(* a fulfil is only fulfilled once *)
+
+Theorem is_fulfil_once:
+  !tr i j t cid cid'. wf_trace tr
+  /\ SUC i < LENGTH tr
+  /\ is_fulfil cid t (FST $ EL i tr) (FST $ EL (SUC i) tr)
+  /\ SUC j < LENGTH tr /\ i <> j
+  ==> ~is_fulfil cid' t (FST $ EL j tr) (FST $ EL (SUC j) tr)
+Proof
+  cheat
+QED
+
+(*
+ * exclusive store and read pairs
+ *)
+
+(* TODO correct return value of bir_get_current_statement *)
+Definition is_read_xcl_def:
+  is_read_xcl cid t sys1 sys2 <=>
+  ?st st' p p' var mem_e a_e en ty.
+    Core cid p st IN sys1
+    /\ Core cid p' st' IN sys2
+    (* /\ st'.bst_pc = bir_pc_next *)
+    /\ bir_get_current_statement p st.bst_pc
+     = SOME $ BStmtB $ BStmt_Assign var $ BExp_Load mem_e a_e en ty
+End
+
+(* TODO correct return value of bir_get_current_statement *)
+Definition is_fulfil_xcl_def:
+  is_fulfil_xcl cid t sys1 sys2 <=>
+    is_fulfil cid t sys1 sys2
+  /\ ?st st' p p' var mem_e a_e en v_e.
+    Core cid p st IN sys1
+    /\ Core cid p' st' IN sys2
+    (* /\ st'.bst_pc = bir_pc_next *)
+    /\ bir_get_current_statement p st.bst_pc
+      = SOME $ BStmtB $ BStmt_Assign var $ BExp_Store mem_e a_e en v_e
+End
+
+(* only exclusive loads set the exclusive bank *)
+
+Theorem xclb_NONE_SOME_is_read_xclb:
+  !t v cid p p' st st' i tr. wf_trace tr /\ SUC i < LENGTH tr
+  /\ Core cid p st IN FST $ EL i tr
+  /\ Core cid p' st' IN FST $ EL (SUC i) tr
+  (* TODO /\ st'.xclb = SOME <| time := t ; view = v |>
+          /\ st.xclb = NONE *)
+  ==> ?t. is_read_xcl cid t (FST $ EL i tr) (FST $ EL (SUC i) tr)
+Proof
+  cheat
+QED
+
+(* an exclusive store has an earlier exclusive load *)
+
+Theorem is_fulfil_xcl_is_read_xcl:
+  !i tr cid p st t. wf_trace tr /\ SUC i < LENGTH tr
+  /\ is_fulfil_xcl cid t (FST $ EL i tr) (FST $ EL (SUC i) tr)
+  /\ Core cid p st IN FST $ EL (SUC i) tr
+  ==> ?j. j < i
+    /\ is_read_xcl cid t (FST $ EL j tr) (FST $ EL (SUC j) tr)
+    /\ !k p' st'. j < k /\ k <= i /\ Core cid p' st' IN FST $ EL k tr
+    ==> ARB
+      (* TODO the exclusive bank is unmodified *)
+      (* st.xclb = st'.xclb  *)
+Proof
+  rpt strip_tac
+  (* TODO there is a (last) process that sets the exclusive bank *)
+  (* TODO by xclb_NONE_SOME_is_read_xclb, this is an exclusive load *)
   >> cheat
 QED
+
+(*
+ * correctness of spinlock
+ *)
+
+Definition core_runs_prog_def:
+  core_runs_prog cid s prog =
+    ?st. Core cid prog st IN s
+    /\ st = <|
+      bst_pc      := bir_program$bir_pc_first prog
+    ; bst_environ  := bir_env_default $ bir_envty_of_vs $
+                        bir_varset_of_program prog
+    ; bst_status := BST_Running
+    ; bst_viewenv := FEMPTY
+    ; bst_coh := \x.0
+    ; bst_v_rOld := 0
+    ; bst_v_CAP := 0
+    ; bst_v_rNew := 0
+    ; bst_v_wNew := 0
+    ; bst_v_wOld := 0
+    ; bst_prom := []
+    ; bst_inflight := []
+    ; bst_fwdb := (\l. <| time:= 0; view:=0; xcl:=F |>)
+    ; bst_counter := 0
+    (* TODO st.bst_xclb = NONE *)
+  |>
+End
+
+Definition core_runs_spinlock_def:
+  core_runs_spinlock cid s =
+    core_runs_prog cid s (bir_spinlock_prog:string bir_program_t)
+End
+
+Definition cores_run_spinlock_def:
+  cores_run_spinlock s =
+    !cid p st. Core cid p st IN s
+      ==> core_runs_spinlock cid s
+End
+
+(* spinlock cores fulfil to the mutex address *)
+(* TODO add mutex address *)
+Theorem is_fulfil_to:
+  !tr cid. wf_trace tr
+  /\ core_runs_spinlock cid (FST $ HD tr)
+  ==> ARB
+Proof
+  cheat
+QED
+
+
+(* Theorem 4 : any exclusive fulfil reads from timestamp 0 onwards *)
+
+Theorem cores_run_spinlock_is_fulfil_xcl_initial_xclb:
+  !tr cid t i s p st. wf_trace tr
+  /\ core_runs_spinlock cid $ FST $ HD tr
+  /\ is_fulfil_xcl cid t (FST $ EL i tr) s
+  /\ Core cid p st IN (FST $ EL i tr)
+  ==> ?x. (* TODO st.bst_xclb = SOME x /\ *) x.time = 0
+Proof
+  cheat
+QED
+
+(* any exiting core must have fulfiled exclusively *)
+
+Theorem core_runs_spinlock_IS_NONE_bst_pc_is_fulfil_xcl:
+  !tr cid p st. wf_trace tr
+  /\ core_runs_spinlock cid (FST $ HD tr)
+  /\ Core cid p st IN (FST $ LAST tr)
+  /\ IS_NONE $ bir_get_current_statement p st.bst_pc
+  ==> ?i t. SUC i < LENGTH tr
+    /\ is_fulfil_xcl cid t (FST $ EL i tr) (FST $ EL (SUC i) tr)
+Proof
+  cheat
+QED
+
+(* distinct exclusive fulfils enforce an ordering on their timestamps *)
+
+Theorem core_runs_spinlock_is_fulfil_xcl_timestamp_order:
+  !tr cid cid' t t' i j i' j' t t'. wf_trace tr
+  /\ core_runs_spinlock cid (FST (HD tr))
+  /\ core_runs_spinlock cid' (FST (HD tr))
+  /\ is_fulfil_xcl cid t (FST (EL i tr)) (FST (EL (SUC i) tr))
+  /\ is_fulfil_xcl cid' t' (FST (EL i' tr)) (FST (EL (SUC i') tr))
+  /\ is_promise cid t (SND (EL j tr)) (SND (EL (SUC j) tr))
+    (FST (EL j tr)) (FST (EL (SUC j) tr))
+  /\ is_promise cid' t' (SND (EL j' tr)) (SND (EL (SUC j') tr))
+    (FST (EL j' tr)) (FST (EL (SUC j') tr))
+  /\ i <> i' /\ j < i /\ j' < i' /\ SUC i' < LENGTH tr
+  ==> ~(t < t')
+Proof
+  rpt strip_tac
+  >> drule_all_then assume_tac wf_trace_parstep_EL
+  >> drule_then (rev_drule_then $ drule_then assume_tac)
+    cores_run_spinlock_is_fulfil_xcl_initial_xclb
+  >> drule_then (drule_then $ drule_then assume_tac)
+    cores_run_spinlock_is_fulfil_xcl_initial_xclb
+  >> gvs[parstep_nice_def,parstep_cases]
+  (* contradiction with atomic predicate and exclusivity bank *)
+  >> cheat
+QED
+
+(* Theorem 5 only one core can leave the lock region *)
+(* TODO add assumption on mutex address for other cores *)
+Theorem core_runs_spinlock_correct:
+  !tr cid cid' t i s p p' st st'. wf_trace tr
+  /\ core_runs_spinlock cid $ FST $ HD tr
+  /\ core_runs_spinlock cid' $ FST $ HD tr
+  /\ Core cid p st IN (FST $ LAST tr)
+  /\ Core cid' p' st' IN (FST $ LAST tr)
+  /\ IS_NONE $ bir_get_current_statement p st.bst_pc
+  /\ IS_NONE $ bir_get_current_statement p' st'.bst_pc
+  ==> cid = cid'
+Proof
+  rpt strip_tac
+  >> drule_then assume_tac wf_trace_NOT_NULL
+  >> drule_then drule core_runs_spinlock_IS_NONE_bst_pc_is_fulfil_xcl
+  >> rpt $ disch_then $ dxrule
+  >> drule_then rev_drule core_runs_spinlock_IS_NONE_bst_pc_is_fulfil_xcl
+  >> rpt $ disch_then $ dxrule
+  >> rw[]
+  >> Cases_on `i = i'`
+  >- (
+    gvs[is_fulfil_xcl_def]
+    >> dxrule is_fulfil_same
+    >> rpt $ disch_then dxrule
+    >> fs[]
+  )
+  >> Cases_on `t = t'`
+  >- (
+    Cases_on `i < i'`
+    >> gvs[is_fulfil_xcl_def]
+    >> dxrule is_fulfil_once
+    >> disch_then $ dxrule_at_then (Pos $ el 2) assume_tac >> gs[LESS_EQ]
+  )
+  >> rev_drule_then assume_tac $ cj 1 $ iffLR is_fulfil_xcl_def
+  >> drule_then assume_tac $ cj 1 $ iffLR is_fulfil_xcl_def
+  >> ntac 2 $ drule_then (dxrule_at Any) is_fulfil_is_promise
+  >> rw[]
+  >> qmatch_assum_rename_tac `j' < i'`
+  >> qmatch_assum_rename_tac `j < i`
+  >> Cases_on `j' = j`
+  >- (
+    gvs[]
+    >> dxrule is_promise_same
+    >> rpt $ disch_then dxrule
+    >> fs[]
+  )
+  >> `~(t < t')` by (
+    drule_then rev_drule core_runs_spinlock_is_fulfil_xcl_timestamp_order
+    >> rpt $ disch_then drule
+    >> fs[]
+  )
+  >> `~(t' < t)` by (
+    drule_then drule core_runs_spinlock_is_fulfil_xcl_timestamp_order
+    >> rpt $ disch_then rev_drule
+    >> fs[]
+  )
+  >> fs[]
+QED
+
+(*
+fetch "-" "bir_spinlock_prog_def"
+bir_spinlock_progbin_def
+*)
 
 val _ = export_theory();
